src/lib/kuiper/Kuiper.Kernel.Sync.fsti
@@ -1,0 +1,23 @@
+module Kuiper.Kernel.Sync
+#lang-pulse
+open Pulse.Lib.Core
+open Kuiper.Common
+open Kuiper.ForEvery
+open Kuiper.Base
+open Kuiper.SizeT
+include Kuiper.Kernel.Base
+include Kuiper.Kernel.Desc
+open FStar.Tactics.Typeclasses
+
+(* A model for launch_kernel_sync *)
+
+noextract
+fn launch_kernel_full_sync
+  (#full_pre #full_post : slprop)
+  (k : kernel_desc full_pre full_post)
+  requires
+    cpu **
+    on gpu_loc full_pre
+  ensures
+    cpu **
+    on gpu_loc full_post
